feat: correctness for `Fin.foldl` and `Fin.foldr`

Std/Data/Fin/Basic.lean
@@ -3,7 +3,8 @@ Copyright (c) 2017 Robert Y. Lewis. All rights reserved.
 Released under Apache 2.0 license as described in the file LICENSE.
 Authors: Robert Y. Lewis, Keeley Hoek, Mario Carneiro
 -/
-import Std.Data.Nat.Init.Lemmas
+import Std.Data.Nat.Basic
+import Std.Data.Array.Init.Lemmas
 
 namespace Fin
 
@@ -48,6 +49,12 @@ def natAdd (n) (i : Fin m) : Fin (n + m) := ⟨n + i, Nat.add_lt_add_left i.2 _�
 
 /-- `min n m` as an element of `Fin (m + 1)` -/
 def clamp (n m : Nat) : Fin (m + 1) := ⟨min n m, Nat.lt_succ_of_le (Nat.min_le_right ..)⟩
+
+/-- `enum n` is the array of all elements of `Fin n` in order -/
+def enum (n) : Array (Fin n) := Array.ofFn id
+
+/-- `list n` is the list of all elements of `Fin n` in order -/
+def list (n) : List (Fin n) := (enum n).data
 
 /-- Folds over `Fin n` from the left: `foldl 3 f x = f (f (f x 0) 1) 2`. -/
 @[inline] def foldl (n) (f : α → Fin n → α) (init : α) : α := loop init 0 where
