Std/Data/List/Lemmas.lean
@@ -5,7 +5,7 @@ Authors: Parikshit Khanna, Jeremy Avigad, Leonardo de Moura, Floris van Doorn, M
 -/
 import Std.Control.ForInStep.Lemmas
 import Std.Data.Bool
-import Std.Data.Fin.Basic
+import Std.Data.Nat.Lemmas
 import Std.Data.List.Basic
 import Std.Data.Option.Lemmas
 import Std.Classes.BEq
@@ -713,7 +713,7 @@ are often used for theorems about `Array.pop`.  -/
   | x::xs => by simp
 
 @[simp] theorem get_dropLast : ∀ (xs : List α) (i : Fin xs.dropLast.length),
-    xs.dropLast.get i = xs.get (i.castLE (xs.length_dropLast ▸ Nat.sub_le ..))
+    xs.dropLast.get i = xs.get ⟨i, Nat.lt_of_lt_of_le i.isLt (length_dropLast .. ▸ Nat.pred_le _)⟩
   | _::_::_, ⟨0, _⟩ => rfl
   | _::_::_, ⟨i+1, _⟩ => get_dropLast _ ⟨i, _⟩
 
